cleanq/crb: rename weak frame condition
Signed-off-by: Roni Häcki <roni.haecki@inf.ethz.ch>

CleanQ/CleanQ_CRBModel.thy
@@ -47,16 +47,16 @@ text \<open>
   stays the same. In order to model this, we have to weaken the frame condition which
   we up to now implicitly used. \<close>
 
-definition frame_rb_weak_x :: "'a CleanQ_RB_State \<Rightarrow> 'a CleanQ_RB_State \<Rightarrow> bool"
-  where "frame_rb_weak_x st' st \<longleftrightarrow> rSX st = rSX st' \<and> frame_rb_weak_left (rTXY st') (rTXY st) \<and> 
+definition CleanQ_RB_frame_weak_x :: "'a CleanQ_RB_State \<Rightarrow> 'a CleanQ_RB_State \<Rightarrow> bool"
+  where "CleanQ_RB_frame_weak_x st' st \<longleftrightarrow> rSX st = rSX st' \<and> frame_rb_weak_left (rTXY st') (rTXY st) \<and> 
                                     frame_rb_weak_right (rTYX st') (rTYX st) \<and> 
                                     rSY st' \<union> set (rb_delta_tail_st (rTXY st') (rTXY st)) = (set (rb_delta_head_st (rTYX st') (rTYX st)) \<union> 
                                     rSY st) \<and> distinct (rb_delta_head_st (rTYX st') (rTYX st)) \<and> 
                                     rSY st \<inter> set (rb_delta_head_st (rTYX st') (rTYX st)) = {}" 
 
 
-definition frame_rb_weak_y :: "'a CleanQ_RB_State \<Rightarrow> 'a CleanQ_RB_State \<Rightarrow> bool"
-  where "frame_rb_weak_y st' st \<longleftrightarrow> rSY st = rSY st' \<and> frame_rb_weak_left (rTYX st') (rTYX st) \<and>
+definition CleanQ_RB_frame_weak_y :: "'a CleanQ_RB_State \<Rightarrow> 'a CleanQ_RB_State \<Rightarrow> bool"
+  where "CleanQ_RB_frame_weak_y st' st \<longleftrightarrow> rSY st = rSY st' \<and> frame_rb_weak_left (rTYX st') (rTYX st) \<and>
                                     frame_rb_weak_right (rTXY st') (rTXY st) \<and>
                                     rSX st' \<union> set (rb_delta_tail_st (rTYX st') (rTYX st)) = (set (rb_delta_head_st (rTXY st') (rTXY st)) \<union> 
                                     rSX st) \<and> distinct (rb_delta_head_st (rTXY st') (rTXY st)) \<and> 
@@ -64,83 +64,83 @@ definition frame_rb_weak_y :: "'a CleanQ_RB_State \<Rightarrow> 'a CleanQ_RB_Sta
 
 
 lemma frame_rb_s_w_x:
- "frame_rb_strong st' st \<Longrightarrow> frame_rb_weak_x st' st"
-  unfolding frame_rb_weak_x_def frame_rb_strong_def frame_rb_weak_left_def
+ "frame_rb_strong st' st \<Longrightarrow> CleanQ_RB_frame_weak_x st' st"
+  unfolding CleanQ_RB_frame_weak_x_def frame_rb_strong_def frame_rb_weak_left_def
   frame_rb_weak_right_def rb_delta_tail_st_def rb_delta_head_st_def
   by (simp add: I4_rb_valid_def rb_delta_head_def rb_delta_tail_def rb_incr_head_n_delta_def 
       rb_incr_head_n_delta_map_def rb_incr_tail_n_delta_def rb_incr_tail_n_delta_map_def)
 
 lemma frame_rb_s_w_y:
-  "frame_rb_strong dev' dev \<Longrightarrow> frame_rb_weak_y dev' dev"
-  unfolding frame_rb_weak_y_def frame_rb_strong_def frame_rb_weak_left_def
+  "frame_rb_strong dev' dev \<Longrightarrow> CleanQ_RB_frame_weak_y dev' dev"
+  unfolding CleanQ_RB_frame_weak_y_def frame_rb_strong_def frame_rb_weak_left_def
   frame_rb_weak_right_def rb_delta_tail_st_def rb_delta_head_st_def
   by (simp add: I4_rb_valid_def rb_delta_head_def rb_delta_tail_def rb_incr_head_n_delta_def 
       rb_incr_head_n_delta_map_def rb_incr_tail_n_delta_def rb_incr_tail_n_delta_map_def)
   
 lemma frame_weak_x_tl_delta: 
   assumes Inv: "CleanQ_RB_Invariants K rb'" and
-          frame: "frame_rb_weak_x rb' rb"
+          frame: "CleanQ_RB_frame_weak_x rb' rb"
   shows"map (the \<circ> ring (rTXY rb')) (rb_valid_entries (rTXY rb')) =
         rb_delta_tail_st (rTXY rb') (rTXY rb) @ map (the \<circ> ring (rTXY rb)) (rb_valid_entries (rTXY rb))"
   unfolding rb_delta_tail_st_def rb_incr_tail_n_delta_map_def rb_incr_tail_n_delta_def
-  by (metis (no_types, hide_lams) frame frame_rb_weak_x_def rb_delta_tail_incr rb_delta_tail_st_def 
+  by (metis (no_types, hide_lams) frame CleanQ_RB_frame_weak_x_def rb_delta_tail_incr rb_delta_tail_st_def 
       rb_incr_tail_n_delta_def rb_incr_tail_n_delta_map_def) 
 
 lemma frame_weak_y_tl_delta: 
   assumes Inv: "CleanQ_RB_Invariants K rb'" and
-          frame: "frame_rb_weak_y rb' rb"
+          frame: "CleanQ_RB_frame_weak_y rb' rb"
   shows"map (the \<circ> ring (rTYX rb')) (rb_valid_entries (rTYX rb')) =
         rb_delta_tail_st (rTYX rb') (rTYX rb) @ map (the \<circ> ring (rTYX rb)) (rb_valid_entries (rTYX rb))"
   unfolding rb_delta_tail_st_def rb_incr_tail_n_delta_map_def rb_incr_tail_n_delta_def
-  by (metis (no_types, hide_lams) frame frame_rb_weak_y_def rb_delta_tail_incr rb_delta_tail_st_def 
+  by (metis (no_types, hide_lams) frame CleanQ_RB_frame_weak_y_def rb_delta_tail_incr rb_delta_tail_st_def 
       rb_incr_tail_n_delta_def rb_incr_tail_n_delta_map_def) 
 
 lemma frame_weak_x_hd_delta:
   assumes Inv: "CleanQ_RB_Invariants K rb'" and
-          frame: "frame_rb_weak_x rb' rb"
+          frame: "CleanQ_RB_frame_weak_x rb' rb"
   shows"map (the \<circ> ring (rTYX rb')) (rb_valid_entries (rTYX rb')) @ rb_delta_head_st (rTYX rb') (rTYX rb) =
         map (the \<circ> ring (rTYX rb)) (rb_valid_entries (rTYX rb))"
   unfolding rb_delta_head_st_def rb_incr_head_n_delta_map_def rb_incr_head_n_delta_def
-  using frame rb_delta_head_incr unfolding frame_rb_weak_x_def
+  using frame rb_delta_head_incr unfolding CleanQ_RB_frame_weak_x_def
   by (metis rb_delta_head_st_def rb_incr_head_n_delta_def rb_incr_head_n_delta_map_def) 
 
 
 lemma frame_weak_y_hd_delta:
   assumes Inv: "CleanQ_RB_Invariants K rb'" and
-          frame: "frame_rb_weak_y rb' rb"
+          frame: "CleanQ_RB_frame_weak_y rb' rb"
   shows"map (the \<circ> ring (rTXY rb')) (rb_valid_entries (rTXY rb')) @ rb_delta_head_st (rTXY rb') (rTXY rb) =
         map (the \<circ> ring (rTXY rb)) (rb_valid_entries (rTXY rb))"
   unfolding rb_delta_head_st_def rb_incr_head_n_delta_map_def rb_incr_head_n_delta_def
-  using frame rb_delta_head_incr unfolding frame_rb_weak_y_def
+  using frame rb_delta_head_incr unfolding CleanQ_RB_frame_weak_y_def
   by (metis rb_delta_head_st_def rb_incr_head_n_delta_def rb_incr_head_n_delta_map_def) 
 
 lemma frame_weak_x_sy_delta:
   assumes Inv: "CleanQ_RB_Invariants K rb'" and
-          frame: "frame_rb_weak_x rb' rb"
+          frame: "CleanQ_RB_frame_weak_x rb' rb"
         shows "rSY rb' \<union> set (rb_delta_tail_st (rTXY rb') (rTXY rb)) = set (rb_delta_head_st (rTYX rb') (rTYX rb)) \<union> rSY rb"
-  using frame unfolding frame_rb_weak_x_def
+  using frame unfolding CleanQ_RB_frame_weak_x_def
   by linarith
 
 lemma frame_weak_y_sx_delta:
   assumes Inv: "CleanQ_RB_Invariants K rb'" and
-          frame: "frame_rb_weak_y rb' rb"
+          frame: "CleanQ_RB_frame_weak_y rb' rb"
         shows "rSX rb' \<union> set (rb_delta_tail_st (rTYX rb') (rTYX rb)) = set (rb_delta_head_st (rTXY rb') (rTXY rb)) \<union> rSX rb"
-  using frame unfolding frame_rb_weak_y_def
+  using frame unfolding CleanQ_RB_frame_weak_y_def
   by linarith
 
 lemma frame_weak_x_sy:
   assumes Inv: "CleanQ_RB_Invariants K rb'" and
-          frame: "frame_rb_weak_x rb' rb"
+          frame: "CleanQ_RB_frame_weak_x rb' rb"
   shows "(rSY rb) \<inter> set (rb_delta_head_st (rTYX rb') (rTYX rb)) = {}"
-  using frame unfolding frame_rb_weak_x_def
+  using frame unfolding CleanQ_RB_frame_weak_x_def
   by blast
 
 
 lemma frame_weak_y_sy:
   assumes Inv: "CleanQ_RB_Invariants K rb'" and
-          frame: "frame_rb_weak_y rb' rb"
+          frame: "CleanQ_RB_frame_weak_y rb' rb"
   shows "(rSX rb) \<inter> set (rb_delta_head_st (rTXY rb') (rTXY rb)) = {}"
-  using frame unfolding frame_rb_weak_y_def
+  using frame unfolding CleanQ_RB_frame_weak_y_def
   by blast
 
 
@@ -149,21 +149,21 @@ text \<open>Finally we show that the RB weak frame condition refines the List we
 lemma frame_rb_weak_x_list_weak:
   fixes rb rb' K
   assumes I1: "CleanQ_RB_Invariants K rb'"
-      and frame: "frame_rb_weak_x rb' rb"
+      and frame: "CleanQ_RB_frame_weak_x rb' rb"
     shows "frame_list_weak (lTXY (CleanQ_RB2List rb'), lSY (CleanQ_RB2List rb'), lTYX (CleanQ_RB2List rb'), lSX (CleanQ_RB2List rb')) 
                            (lTXY (CleanQ_RB2List rb), lSY (CleanQ_RB2List rb), lTYX (CleanQ_RB2List rb), lSX (CleanQ_RB2List rb))"
   unfolding CleanQ_RB2List_def CleanQ_RB_list_def
-  using I1 frame frame_rb_weak_x_def frame_weak_x_hd_delta frame_weak_x_tl_delta by fastforce
+  using I1 frame CleanQ_RB_frame_weak_x_def frame_weak_x_hd_delta frame_weak_x_tl_delta by fastforce
  
 
 lemma frame_rb_weak_y_list_weak:
   fixes rb rb' K
   assumes I1: "CleanQ_RB_Invariants K rb'"
-      and frame: "frame_rb_weak_y rb' rb"
+      and frame: "CleanQ_RB_frame_weak_y rb' rb"
     shows "frame_list_weak (lTYX (CleanQ_RB2List rb'), lSX (CleanQ_RB2List rb'), lTXY (CleanQ_RB2List rb'), lSY (CleanQ_RB2List rb')) 
                            (lTYX (CleanQ_RB2List rb), lSX (CleanQ_RB2List rb), lTXY (CleanQ_RB2List rb), lSY (CleanQ_RB2List rb))"
   unfolding CleanQ_RB2List_def CleanQ_RB_list_def
-  using I1 frame frame_rb_weak_y_def frame_weak_y_hd_delta frame_weak_y_tl_delta by fastforce
+  using I1 frame CleanQ_RB_frame_weak_y_def frame_weak_y_hd_delta frame_weak_y_tl_delta by fastforce
 
 
 
@@ -174,46 +174,46 @@ subsubsection \<open>Weak frame condition preserver invariants\<close>
 
 lemma frame_rb_weak_x_notin_xy_yx_sy:
   fixes rb rb' K
-  assumes frame: "frame_rb_weak_x rb' rb"
+  assumes frame: "CleanQ_RB_frame_weak_x rb' rb"
     and invariants : "CleanQ_RB_Invariants K rb'"
   shows "x \<in> K \<Longrightarrow> x \<notin> set (CleanQ_RB_list (rTYX rb)) \<Longrightarrow> x \<notin> set (CleanQ_RB_list (rTXY rb)) \<Longrightarrow> x \<notin> rSY rb \<Longrightarrow> x \<in> rSX rb'"
-  using assms unfolding frame_rb_weak_x_def CleanQ_RB_Invariants_def
+  using assms unfolding CleanQ_RB_frame_weak_x_def CleanQ_RB_Invariants_def
   by (smt CleanQ_RB_list_def I1_rb_img_def UnCI UnI2 Un_commute Un_iff inf_commute rb_delta_head_incr 
       rb_delta_tail_incr set_append) 
 
 lemma frame_rb_weak_y_notin_xy_yx_sx:
   fixes rb rb' K
-  assumes frame: "frame_rb_weak_y rb' rb"
+  assumes frame: "CleanQ_RB_frame_weak_y rb' rb"
     and invariants : "CleanQ_RB_Invariants K rb'"
   shows "x \<in> K \<Longrightarrow> x \<notin> set (CleanQ_RB_list (rTXY rb)) \<Longrightarrow> x \<notin> set (CleanQ_RB_list (rTYX rb)) \<Longrightarrow> x \<notin> rSX rb \<Longrightarrow> x \<in> rSY rb'"
-  using assms unfolding frame_rb_weak_y_def CleanQ_RB_Invariants_def frame_rb_weak_left_def
+  using assms unfolding CleanQ_RB_frame_weak_y_def CleanQ_RB_Invariants_def frame_rb_weak_left_def
   frame_rb_weak_right_def apply auto
   by (smt CleanQ_RB_list_def I1_rb_img_def UnE Un_commute Un_upper2 frame frame_rb_weak_right_def 
       frame_weak_y_tl_delta invariants rb_delta_head_incr set_append subsetD)
 
 lemma CleanQ_CRB_frame_x_I1 :
   fixes rb rb' K
-  assumes frame: "frame_rb_weak_x rb' rb"
+  assumes frame: "CleanQ_RB_frame_weak_x rb' rb"
     and invariants : "CleanQ_RB_Invariants K rb'"
   shows "I1_rb_img rb K"
-  using assms unfolding frame_rb_weak_x_def I1_rb_img_def CleanQ_RB_Invariants_def
+  using assms unfolding CleanQ_RB_frame_weak_x_def I1_rb_img_def CleanQ_RB_Invariants_def
   frame_rb_weak_left_def frame_rb_weak_right_def
   apply auto
   apply (smt CleanQ_RB_list_def UnE UnI1 Un_upper2 frame frame_weak_x_tl_delta invariants set_append subsetD)
   apply (metis CleanQ_RB_list_def UnCI frame frame_weak_x_tl_delta invariants set_append)
-  apply (smt CleanQ_RB_list_def UnE frame frame_rb_weak_x_def frame_weak_x_tl_delta invariants 
+  apply (smt CleanQ_RB_list_def UnE frame CleanQ_RB_frame_weak_x_def frame_weak_x_tl_delta invariants 
          rb_delta_head_incr set_append subsetD sup_ge1)
   using frame frame_rb_weak_x_notin_xy_yx_sy invariants apply fastforce
   apply (metis (no_types) Un_iff frame frame_rb_weak_x_notin_xy_yx_sy invariants)
-  by (metis CleanQ_RB_list_def UnCI frame frame_rb_weak_x_def rb_delta_head_incr set_append)
+  by (metis CleanQ_RB_list_def UnCI frame CleanQ_RB_frame_weak_x_def rb_delta_head_incr set_append)
   
 
 lemma CleanQ_CRB_frame_y_I1 :
   fixes rb rb' K
-  assumes frame: "frame_rb_weak_y rb' rb"
+  assumes frame: "CleanQ_RB_frame_weak_y rb' rb"
     and invariants : "CleanQ_RB_Invariants K rb'"
   shows "I1_rb_img rb K"
-  using assms unfolding frame_rb_weak_y_def I1_rb_img_def CleanQ_RB_Invariants_def
+  using assms unfolding CleanQ_RB_frame_weak_y_def I1_rb_img_def CleanQ_RB_Invariants_def
   frame_rb_weak_left_def frame_rb_weak_right_def
   apply auto
   apply (smt CleanQ_RB_list_def UnE UnI1 Un_upper2 frame frame_weak_y_tl_delta invariants set_append subsetD)
@@ -227,83 +227,83 @@ lemma CleanQ_CRB_frame_y_I1 :
 
 lemma frame_rb_weak_x_in_deltaxy_notin_txy:
   fixes rb rb' K
-  assumes frame: "frame_rb_weak_x rb' rb"
+  assumes frame: "CleanQ_RB_frame_weak_x rb' rb"
     and invariants : "CleanQ_RB_Invariants K rb'"
   shows "x \<in> set (rb_delta_tail_st (rTXY rb') (rTXY rb)) \<Longrightarrow> x \<notin> set (CleanQ_RB_list (rTXY rb))"
-  using assms unfolding CleanQ_RB_Invariants_def frame_rb_weak_x_def
+  using assms unfolding CleanQ_RB_Invariants_def CleanQ_RB_frame_weak_x_def
   by (metis CleanQ_RB_list_def I3_rb_img_def Int_iff distinct_append insert_absorb insert_not_empty 
       rb_delta_tail_incr) 
 
 
 lemma frame_rb_weak_y_in_deltaxy_notin_txy:
   fixes rb rb' K
-  assumes frame: "frame_rb_weak_y rb' rb"
+  assumes frame: "CleanQ_RB_frame_weak_y rb' rb"
     and invariants : "CleanQ_RB_Invariants K rb'"
   shows "x \<in> set (rb_delta_tail_st (rTYX rb') (rTYX rb)) \<Longrightarrow> x \<notin> set (CleanQ_RB_list (rTYX rb))"
-  using assms unfolding CleanQ_RB_Invariants_def frame_rb_weak_y_def
+  using assms unfolding CleanQ_RB_Invariants_def CleanQ_RB_frame_weak_y_def
   by (metis CleanQ_RB_list_def I3_rb_img_def disjoint_iff_not_equal distinct_append rb_delta_tail_incr) 
 
 lemma frame_rb_weak_x_in_sy_notin_txy:
   fixes rb rb' K
-  assumes frame: "frame_rb_weak_x rb' rb"
+  assumes frame: "CleanQ_RB_frame_weak_x rb' rb"
     and invariants : "CleanQ_RB_Invariants K rb'"
   shows" x \<in> rSY rb \<Longrightarrow> x \<in> set (CleanQ_RB_list (rTXY rb)) \<Longrightarrow> False"
-  using assms unfolding CleanQ_RB_Invariants_def frame_rb_weak_x_def
+  using assms unfolding CleanQ_RB_Invariants_def CleanQ_RB_frame_weak_x_def
   by (smt CleanQ_RB_list_def I2_rb_img_def I3_rb_img_def UnE Un_upper2 disjoint_iff_not_equal distinct_append 
       rb_delta_tail_incr set_append subsetD) 
 
 lemma frame_rb_weak_y_in_sx_notin_tyx:
   fixes rb rb' K
-  assumes frame: "frame_rb_weak_y rb' rb"
+  assumes frame: "CleanQ_RB_frame_weak_y rb' rb"
     and invariants : "CleanQ_RB_Invariants K rb'"
   shows" x \<in> rSX rb \<Longrightarrow> x \<in> set (CleanQ_RB_list (rTYX rb)) \<Longrightarrow> False"
-  using assms unfolding frame_rb_weak_y_def CleanQ_RB_Invariants_def
+  using assms unfolding CleanQ_RB_frame_weak_y_def CleanQ_RB_Invariants_def
   by (smt CleanQ_RB_list_def I2_rb_img_def I3_rb_img_def UnE Un_upper2 disjoint_iff_not_equal 
       distinct_append rb_delta_tail_incr set_append subsetD)
 
 lemma frame_rb_weak_y_in_sx_notin_txy:
   fixes rb rb' K
-  assumes frame: "frame_rb_weak_y rb' rb"
+  assumes frame: "CleanQ_RB_frame_weak_y rb' rb"
     and invariants : "CleanQ_RB_Invariants K rb'"
   shows" x \<in> rSX rb \<Longrightarrow> x \<in> set (CleanQ_RB_list (rTXY rb)) \<Longrightarrow> False"
-  using assms unfolding frame_rb_weak_y_def CleanQ_RB_Invariants_def
+  using assms unfolding CleanQ_RB_frame_weak_y_def CleanQ_RB_Invariants_def
   by (smt CleanQ_RB_list_def I2_rb_img_def UnE Un_commute Un_upper2 disjoint_iff_not_equal frame 
       frame_weak_y_hd_delta frame_weak_y_tl_delta invariants set_append subsetD) 
 
 lemma frame_rb_weak_x_in_txy_notin_tyx:
   fixes rb rb' K
-  assumes frame: "frame_rb_weak_x rb' rb"
+  assumes frame: "CleanQ_RB_frame_weak_x rb' rb"
     and invariants : "CleanQ_RB_Invariants K rb'"  
   shows "x \<in> set (CleanQ_RB_list (rTXY rb)) \<Longrightarrow> x \<in> set (CleanQ_RB_list (rTYX rb)) \<Longrightarrow> False"
-  using assms unfolding frame_rb_weak_x_def CleanQ_RB_Invariants_def
+  using assms unfolding CleanQ_RB_frame_weak_x_def CleanQ_RB_Invariants_def
   by (smt CleanQ_RB_list_def I2_rb_img_def I3_rb_img_def Set.set_insert UnE disjoint_insert(1) 
       distinct_append rb_delta_head_incr rb_delta_tail_incr set_append subsetD sup.cobounded2 sup.commute)
 
 lemma frame_rb_weak_x_sx_notin_yx:
   fixes rb rb' K
-  assumes frame: "frame_rb_weak_x rb' rb"
+  assumes frame: "CleanQ_RB_frame_weak_x rb' rb"
     and invariants : "CleanQ_RB_Invariants K rb'" 
   shows "x \<in> rSX rb' \<Longrightarrow> x \<in> set (CleanQ_RB_list (rTYX rb)) \<Longrightarrow> False"
-  using assms unfolding frame_rb_weak_x_def CleanQ_RB_Invariants_def
+  using assms unfolding CleanQ_RB_frame_weak_x_def CleanQ_RB_Invariants_def
   by (smt CleanQ_RB_list_def I2_rb_img_def Int_iff Set.set_insert Un_iff disjoint_insert(1) 
       inf_sup_absorb rb_delta_head_incr rb_delta_tail_incr set_append)
 
 lemma frame_rb_weak_y_sy_notin_xy:
   fixes rb rb' K
-  assumes frame: "frame_rb_weak_y rb' rb"
+  assumes frame: "CleanQ_RB_frame_weak_y rb' rb"
     and invariants : "CleanQ_RB_Invariants K rb'" 
   shows "x \<in> rSY rb' \<Longrightarrow> x \<in> set (CleanQ_RB_list (rTXY rb)) \<Longrightarrow> False"
-  using assms unfolding frame_rb_weak_y_def CleanQ_RB_Invariants_def
+  using assms unfolding CleanQ_RB_frame_weak_y_def CleanQ_RB_Invariants_def
   by (smt CleanQ_RB_list_def I2_rb_img_def UnE disjoint_insert(1) insert_Diff rb_delta_head_incr 
       rb_delta_tail_incr set_append subsetD sup_ge1)
 
 
 lemma CleanQ_CRB_frame_x_I2 :
   fixes rb rb' K
-  assumes frame: "frame_rb_weak_x rb' rb"
+  assumes frame: "CleanQ_RB_frame_weak_x rb' rb"
     and invariants : "CleanQ_RB_Invariants K rb'"
   shows "I2_rb_img rb"
-  using assms unfolding frame_rb_weak_x_def CleanQ_RB_Invariants_def I2_rb_img_def
+  using assms unfolding CleanQ_RB_frame_weak_x_def CleanQ_RB_Invariants_def I2_rb_img_def
   apply auto
   apply (smt CleanQ_RB_list_def UnE UnI1 Un_upper2 disjoint_iff_not_equal frame frame_weak_x_tl_delta 
          invariants set_append subsetD)
@@ -317,10 +317,10 @@ lemma CleanQ_CRB_frame_x_I2 :
  
 lemma CleanQ_CRB_frame_y_I2 :
   fixes rb rb' K
-  assumes frame: "frame_rb_weak_y rb' rb"
+  assumes frame: "CleanQ_RB_frame_weak_y rb' rb"
     and invariants : "CleanQ_RB_Invariants K rb'"
   shows "I2_rb_img rb"
-  using assms unfolding frame_rb_weak_y_def CleanQ_RB_Invariants_def I2_rb_img_def
+  using assms unfolding CleanQ_RB_frame_weak_y_def CleanQ_RB_Invariants_def I2_rb_img_def
   apply auto
   apply (smt CleanQ_RB_list_def UnE Un_commute Un_upper2 disjoint_iff_not_equal frame frame_weak_y_tl_delta 
       invariants set_append subsetD)
@@ -333,54 +333,54 @@ lemma CleanQ_CRB_frame_y_I2 :
 
 lemma CleanQ_CRB_frame_x_I3 :
   fixes rb rb' K
-  assumes frame: "frame_rb_weak_x rb' rb"
+  assumes frame: "CleanQ_RB_frame_weak_x rb' rb"
       and invariants : "CleanQ_RB_Invariants K rb'"
   shows "I3_rb_img rb"
-  using assms unfolding frame_rb_weak_x_def CleanQ_RB_Invariants_def I3_rb_img_def
+  using assms unfolding CleanQ_RB_frame_weak_x_def CleanQ_RB_Invariants_def I3_rb_img_def
   by (smt CleanQ_RB_list_def I2_rb_img_def distinct_append inf_commute inf_left_commute inf_sup_absorb 
       inf_sup_distrib1 rb_delta_head_incr rb_delta_tail_incr set_append)
 
 lemma CleanQ_CRB_frame_y_I3 :
   fixes rb rb' K
-  assumes frame: "frame_rb_weak_y rb' rb"
+  assumes frame: "CleanQ_RB_frame_weak_y rb' rb"
       and invariants : "CleanQ_RB_Invariants K rb'"
   shows "I3_rb_img rb"
-  using assms unfolding frame_rb_weak_y_def CleanQ_RB_Invariants_def I3_rb_img_def
+  using assms unfolding CleanQ_RB_frame_weak_y_def CleanQ_RB_Invariants_def I3_rb_img_def
   by (smt CleanQ_RB_list_def I2_rb_img_def distinct_append inf_commute inf_left_commute inf_sup_absorb 
       inf_sup_distrib1 rb_delta_head_incr rb_delta_tail_incr set_append)
 
 lemma CleanQ_CRB_frame_x_I4 :
   fixes rb rb' K
-  assumes frame: "frame_rb_weak_x rb' rb"
+  assumes frame: "CleanQ_RB_frame_weak_x rb' rb"
       and invariants : "CleanQ_RB_Invariants K rb'"
   shows "I4_rb_valid rb"
-  using assms unfolding frame_rb_weak_x_def CleanQ_RB_Invariants_def I4_rb_valid_def
+  using assms unfolding CleanQ_RB_frame_weak_x_def CleanQ_RB_Invariants_def I4_rb_valid_def
   by (simp add: frame_rb_weak_left_def frame_rb_weak_right_def)
 
   
 lemma CleanQ_CRB_frame_y_I4 :
   fixes rb rb' K
-  assumes frame: "frame_rb_weak_y rb' rb"
+  assumes frame: "CleanQ_RB_frame_weak_y rb' rb"
       and invariants : "CleanQ_RB_Invariants K rb'"
   shows "I4_rb_valid rb"
-  using assms unfolding frame_rb_weak_y_def CleanQ_RB_Invariants_def I4_rb_valid_def
+  using assms unfolding CleanQ_RB_frame_weak_y_def CleanQ_RB_Invariants_def I4_rb_valid_def
   by (simp add: frame_rb_weak_left_def frame_rb_weak_right_def)
   
 lemma CleanQ_CRB_frame_x_I_all :
   fixes rb rb' K
-  assumes frame: "frame_rb_weak_x rb' rb"
+  assumes frame: "CleanQ_RB_frame_weak_x rb' rb"
       and invariants : "CleanQ_RB_Invariants K rb'"
   shows "CleanQ_RB_Invariants K rb"
-  using assms unfolding frame_rb_weak_x_def CleanQ_RB_Invariants_def
+  using assms unfolding CleanQ_RB_frame_weak_x_def CleanQ_RB_Invariants_def
   by (meson CleanQ_CRB_frame_x_I1 CleanQ_CRB_frame_x_I2 CleanQ_CRB_frame_x_I3 CleanQ_CRB_frame_x_I4 
       frame invariants)
 
 lemma CleanQ_CRB_frame_y_I_all :
   fixes rb rb' K
-  assumes frame: "frame_rb_weak_y rb' rb"
+  assumes frame: "CleanQ_RB_frame_weak_y rb' rb"
       and invariants : "CleanQ_RB_Invariants K rb'"
   shows "CleanQ_RB_Invariants K rb"
-  using assms unfolding frame_rb_weak_y_def CleanQ_RB_Invariants_def
+  using assms unfolding CleanQ_RB_frame_weak_y_def CleanQ_RB_Invariants_def
   by (meson CleanQ_CRB_frame_y_I1 CleanQ_CRB_frame_y_I2 CleanQ_CRB_frame_y_I3 CleanQ_CRB_frame_y_I4 
       frame invariants)
 
